theory/Abstract_Communication_Analysis.thy
@@ -32,16 +32,16 @@ definition topo_env_precision :: "topo_env \<Rightarrow> topo_env \<Rightarrow> 
   "\<A> \<sqsubseteq>\<^sub>t \<A>' \<equiv> (\<forall> x . \<A> x \<preceq> \<A>' x)"
 
 definition abstract_send_paths :: "(abstract_value_env \<times> abstract_value_env \<times> exp) \<Rightarrow> var \<Rightarrow> control_path set" where
-  "abstract_send_paths \<A> x\<^sub>c \<equiv> case \<A> of (\<V>, \<C>, e) \<Rightarrow> {\<pi>\<^sub>y;;`x\<^sub>y | \<pi>\<^sub>y x\<^sub>y x\<^sub>e x\<^sub>s\<^sub>c x\<^sub>m e'. 
-    \<V> \<turnstile> e \<down> (\<pi>\<^sub>y, LET x\<^sub>y = SYNC x\<^sub>e in e') \<and>
+  "abstract_send_paths \<A> x\<^sub>c \<equiv> case \<A> of (\<V>, \<C>, e) \<Rightarrow> {\<pi>\<^sub>y;;`x\<^sub>y | \<pi>\<^sub>y x\<^sub>y x\<^sub>e x\<^sub>s\<^sub>c x\<^sub>m e\<^sub>n. 
+    \<V> \<turnstile> e \<down> (\<pi>\<^sub>y, LET x\<^sub>y = SYNC x\<^sub>e in e\<^sub>n) \<and>
     ^Chan x\<^sub>c \<in> \<V> x\<^sub>s\<^sub>c \<and>
     {^Send_Evt x\<^sub>s\<^sub>c x\<^sub>m} \<subseteq> \<V> x\<^sub>e \<and>
     {^\<lparr>\<rparr>} \<subseteq> \<V> x\<^sub>y \<and> \<V> x\<^sub>m \<subseteq> \<C> x\<^sub>c
   }"
 
 definition abstract_recv_paths :: "(abstract_value_env \<times> abstract_value_env \<times> exp) \<Rightarrow> var \<Rightarrow> control_path set" where
-  "abstract_recv_paths \<A> x\<^sub>c \<equiv> case \<A> of (\<V>, \<C>, e) \<Rightarrow> {\<pi>\<^sub>y;;`x\<^sub>y | \<pi>\<^sub>y x\<^sub>y x\<^sub>e x\<^sub>r\<^sub>c e' \<omega>. 
-    \<V> \<turnstile> e \<down> (\<pi>\<^sub>y, LET x\<^sub>y = SYNC x\<^sub>e in e') \<and>
+  "abstract_recv_paths \<A> x\<^sub>c \<equiv> case \<A> of (\<V>, \<C>, e) \<Rightarrow> {\<pi>\<^sub>y;;`x\<^sub>y | \<pi>\<^sub>y x\<^sub>y x\<^sub>e x\<^sub>r\<^sub>c e\<^sub>n \<omega>. 
+    \<V> \<turnstile> e \<down> (\<pi>\<^sub>y, LET x\<^sub>y = SYNC x\<^sub>e in e\<^sub>n) \<and>
     ^Chan x\<^sub>c \<in> \<V> x\<^sub>r\<^sub>c \<and>
     {^Recv_Evt x\<^sub>r\<^sub>c} \<subseteq> \<V> x\<^sub>e \<and>
     {|\<omega>|} \<subseteq> \<V> x\<^sub>y
