theory/Communication_Analysis.thy
@@ -3,31 +3,20 @@ theory Communication_Analysis
 begin
 
 definition send_paths :: "state_pool \<Rightarrow> chan \<Rightarrow> control_path set" where
-  "send_paths \<E> c \<equiv> {\<pi>\<^sub>y ;; `x\<^sub>y | \<pi>\<^sub>y x\<^sub>y x\<^sub>e e \<kappa> \<rho> x\<^sub>s\<^sub>c x\<^sub>m \<rho>\<^sub>e. 
-    \<E> \<pi>\<^sub>y = Some (\<langle>LET x\<^sub>y = SYNC x\<^sub>e in e; \<rho>; \<kappa>\<rangle>) \<and>
+  "send_paths \<E> c \<equiv> {\<pi>\<^sub>y ;; `x\<^sub>y | \<pi>\<^sub>y x\<^sub>y x\<^sub>e e\<^sub>n \<kappa> \<rho> x\<^sub>s\<^sub>c x\<^sub>m \<rho>\<^sub>e. 
+    \<E> \<pi>\<^sub>y = Some (\<langle>LET x\<^sub>y = SYNC x\<^sub>e in e\<^sub>n; \<rho>; \<kappa>\<rangle>) \<and>
     \<rho> x\<^sub>e = Some \<lbrace>Send_Evt x\<^sub>s\<^sub>c x\<^sub>m, \<rho>\<^sub>e\<rbrace> \<and> 
     \<rho>\<^sub>e x\<^sub>s\<^sub>c = Some \<lbrace>c\<rbrace> \<and>
-    \<E> (\<pi>\<^sub>y;;`x\<^sub>y) = Some (\<langle>e; \<rho>(x\<^sub>y \<mapsto> \<lbrace>\<rbrace>); \<kappa>\<rangle>)
+    \<E> (\<pi>\<^sub>y;;`x\<^sub>y) = Some (\<langle>e\<^sub>n; \<rho>(x\<^sub>y \<mapsto> \<lbrace>\<rbrace>); \<kappa>\<rangle>)
   }"
 
 definition recv_paths :: "state_pool \<Rightarrow> chan \<Rightarrow> control_path set" where
-  "recv_paths \<E> c \<equiv> {\<pi>\<^sub>y ;; `x\<^sub>y | \<pi>\<^sub>y x\<^sub>y x\<^sub>e e \<kappa> \<rho> x\<^sub>r\<^sub>c \<rho>\<^sub>e \<omega>. 
-    \<E> \<pi>\<^sub>y = Some (\<langle>LET x\<^sub>y = SYNC x\<^sub>e in e; \<rho>; \<kappa>\<rangle>) \<and> 
+  "recv_paths \<E> c \<equiv> {\<pi>\<^sub>y ;; `x\<^sub>y | \<pi>\<^sub>y x\<^sub>y x\<^sub>e e\<^sub>n \<kappa> \<rho> x\<^sub>r\<^sub>c \<rho>\<^sub>e \<omega>. 
+    \<E> \<pi>\<^sub>y = Some (\<langle>LET x\<^sub>y = SYNC x\<^sub>e in e\<^sub>n; \<rho>; \<kappa>\<rangle>) \<and> 
     \<rho> x\<^sub>e = Some \<lbrace>Recv_Evt x\<^sub>r\<^sub>c, \<rho>\<^sub>e\<rbrace> \<and> 
     \<rho>\<^sub>e x\<^sub>r\<^sub>c = Some \<lbrace>c\<rbrace> \<and>
-    \<E> (\<pi>\<^sub>y;;`x\<^sub>y) = Some (\<langle>e; \<rho>(x\<^sub>y \<mapsto> \<omega>); \<kappa>\<rangle>)
+    \<E> (\<pi>\<^sub>y;;`x\<^sub>y) = Some (\<langle>e\<^sub>n; \<rho>(x\<^sub>y \<mapsto> \<omega>); \<kappa>\<rangle>)
   }"
-
-
-(*
-fun proc_legacy' where 
-  "proc_legacy' [] = []" |
-  "proc_legacy' (.x # xs) = (.x # xs)" |
-  "proc_legacy' (_ # xs) = proc_legacy' xs"
-
-fun proc_legacy :: "control_path \<Rightarrow> control_path" where
-  "proc_legacy \<pi> = rev (proc_legacy' (rev \<pi>))"
-*)
 
 
 inductive same_proc :: "control_path \<Rightarrow> control_path \<Rightarrow> bool" (infix "\<cong>" 55) where
